Introducing generics
Work in progress:
- lang.v is mostly updated, but there is a few quirks
  + need to change VarT into GenericT
  + need to correctly deal with runtime check (maybe existential ?)
- heap.v is fine
- interp.v is ok until inheritance -> inclusion
  + I think Nick was right about interp_class being inaccurate
  + that where I'll work next

theories/interp.v
@@ -4,7 +4,7 @@
  * This source code is licensed under the MIT license found in the
  * LICENSE file in the root directory of this source tree.
  *)
-From stdpp Require Import base strings gmap stringmap fin_maps.
+From stdpp Require Import base strings gmap stringmap fin_maps natmap.
 From iris.base_logic Require Import upred derived.
 From iris.base_logic.lib Require Import iprop own.
 From iris.algebra Require Import ofe cmra gmap_view.
@@ -19,7 +19,7 @@ Record interp Σ := Interp {
     interp_persistent v : Persistent (interp_car v)
   }.
 
-Lemma interp_car_unfold : ∀ Σ c p, @interp_car Σ (Interp _ c p) = c.
+Lemma interp_car_simpl : ∀ Σ c p, @interp_car Σ (Interp _ c p) = c.
 Proof.
   by intros.
 Qed.
@@ -73,10 +73,6 @@ Section proofs.
   Local Notation "lty <:< rty" := (@lty_sub _ lty rty) (at level 70, no associativity).
 
   (* now, let's interpret some types ! *)
-  Definition interp_null_car (v: value) : iProp Σ := ⌜v = NullV⌝%I.
-  Definition interp_null_persistent v : Persistent (interp_null_car v).
-  Proof. by apply _. Qed.
-
   Definition interp_null : interp Σ :=
     Interp (λ(v: value), ⌜v = NullV⌝%I).
 
@@ -95,82 +91,195 @@ Section proofs.
   Definition interp_nothing : interp Σ :=
     Interp (λ (_: value), False%I).
 
-  Notation ty_interpO := (lang_ty -d> sem_typeO Σ).
+   Notation ty_interpO := (lang_ty -d> listO (interpO Σ) -n> sem_typeO Σ).
 
-  Definition interp_fields (rec: ty_interpO) (ftys: stringmap lang_ty) :
+   Lemma ty_interpO_ne : ∀ (rec: ty_interpO) ty, NonExpansive (rec ty).
+   Proof.
+     move => rec ty.
+     apply _.
+   Qed.
+
+  Definition interp_fields (env: list (interp Σ)) (ftys: stringmap lang_ty) (rec: ty_interpO) :
     gmapO string (laterO (sem_typeO Σ)) :=
-    let f := λ (typ: lang_ty), Next (rec typ) in
+    let f := λ (typ: lang_ty), Next (rec typ env) in
     @fmap _ _ _ (later (sem_typeO Σ)) f ftys
   .
 
-  Lemma interp_fields_contractive ftys:
-    Contractive (λ f, interp_fields f ftys).
+  Lemma interp_fields_contractive ftys env: Contractive (interp_fields env ftys).
   Proof.
-    move => n i1 i2 hdist.
-    rewrite /interp_fields.
+    rewrite /interp_fields => n i1 i2 hdist.
     apply gmap_fmap_ne_ext => k ty hin.
     f_contractive.
-    by destruct n.
+    by f_equiv.
+  Qed.
+
+  Lemma interp_fields_ne ftys (rec: ty_interpO):
+    NonExpansive (λ env, interp_fields env ftys rec).
+  Proof.
+    rewrite /interp_fields => n l1 l2 h f.
+    f_equiv.
+    apply gmap_fmap_ne_ext => k ty hin.
+    f_equiv.
+    by apply ty_interpO_ne.
   Qed.
 
   (* interpret a class type given the tag and the
      interpretation of their fields *)
-  Definition interp_class (cname : tag) (rec : ty_interpO) : interp Σ :=
+  Definition interp_class (cname : tag) (env: list (interp Σ)) (rec : ty_interpO) : interp Σ :=
     Interp (
       λ (w : value),
       (∃ ℓ t (fields:stringmap lang_ty),
       ⌜w = LocV ℓ ∧ inherits t cname ∧ has_fields t fields⌝ ∗
-      (ℓ ↦ (t , interp_fields rec fields)))%I
+      (ℓ ↦ (t , interp_fields env fields rec)))%I
     ).
 
-  Definition interp_nonnull (rec : ty_interpO) : interp Σ :=
+  Definition interp_nonnull (env: list (interp Σ)) (rec : ty_interpO) : interp Σ :=
     Interp (
       λ (v : value),
       ((interp_int v) ∨
       (interp_bool v) ∨
-      (∃ t, interp_class t rec v))%I
+      (∃ t, interp_class t env rec v))%I
     ).
 
-  Definition interp_mixed (rec: ty_interpO) : interp Σ :=
-    Interp (λ (v: value), (interp_nonnull rec v ∨ interp_null v)%I).
+  Definition interp_mixed (env: list (interp Σ)) (rec: ty_interpO) : interp Σ :=
+    Interp (λ (v: value), (interp_nonnull env rec v ∨ interp_null v)%I).
+
+  Definition interp_tvar (env: list (interp Σ)) (tv: nat) : interp Σ :=
+    List.nth tv env interp_nothing.
 
   (* we use a blend of Coq/Iris recursion, the
      Coq recursion lets us handle simple structural
      cases, and we use Iris' recursion to deal with
-     the more complicated case of class types *)
-  Definition interp_type_pre (rec : ty_interpO) : ty_interpO :=
-    λ (typ : lang_ty),
-    (fix go (typ : lang_ty) : interp Σ :=
-    match typ with
-    | IntT => interp_int
-    | BoolT => interp_bool
-    | NothingT => interp_nothing
-    | MixedT => interp_mixed rec
-    | ClassT t => interp_class t rec
-    | NullT => interp_null
-    | NonNullT => interp_nonnull rec
-    | UnionT A B => interp_union (go A) (go B)
-    | InterT A B => interp_inter (go A) (go B)
-    end) typ.
+     the more complicated case of class types.
+  *)
+  Section interp_type_pre_rec.
+    Variable (env: listO (interpO Σ)).
+    Variable (rec: ty_interpO).
 
-  Lemma interp_class_contractive cname:
-    Contractive (interp_class cname).
+    Fixpoint go (typ: lang_ty) : interp Σ :=
+      match typ with
+      | IntT => interp_int
+      | BoolT => interp_bool
+      | NothingT => interp_nothing
+      | MixedT => interp_mixed env rec
+      | ClassT t targs =>
+          let env : list (interp Σ) := List.map go targs in
+          interp_class t env rec
+      | NullT => interp_null
+      | NonNullT => interp_nonnull env rec
+      | UnionT A B => interp_union (go A) (go B)
+      | InterT A B => interp_inter (go A) (go B)
+      | VarT tv => interp_tvar env tv
+      end.
+  End interp_type_pre_rec.
+
+  Lemma interp_class_ne cname (rec: ty_interpO) :
+    NonExpansive (λ env, interp_class cname env rec).
+  Proof.
+    move => n x y h.
+    rewrite /interp_class => v.
+    rewrite !interp_car_simpl.
+    do 7 f_equiv.
+    rewrite mapsto_eq /mapsto_def /loc_mapsto_def.
+    do 3 f_equiv.
+    by apply interp_fields_ne.
+  Qed.
+
+  Definition itp_rec (env: listO (interpO Σ)) (rec: ty_interpO) (ty: lang_ty)
+      : sem_typeO Σ := go env rec ty.
+
+  Local Instance itp_ne (rec: ty_interpO) (ty: lang_ty) :
+    NonExpansive (λ (env: listO (interpO Σ)), itp_rec env rec ty).
+  Proof.
+    rewrite /itp_rec.
+    induction ty
+      as [ | | | | cname targs htargs | | | A B hA hB | A B hA hB | tv ]
+      using lang_ty_ind' => //= n x y h.
+    - rewrite /interp_mixed => v.
+      rewrite !interp_car_simpl.
+      f_equiv.
+      do 4 f_equiv.
+      revert v.
+      by apply interp_class_ne.
+    - apply interp_class_ne => //.
+      rewrite Forall_forall in htargs.
+      induction targs as [ | hd tl hi] => //=.
+      f_equiv.
+      { apply htargs; last done.
+        by constructor.
+      }
+      apply hi => ? hIn.
+      apply htargs.
+      now constructor.
+    - rewrite /interp_nonnull => v.
+      rewrite !interp_car_simpl.
+      do 4 f_equiv.
+      revert v; by apply interp_class_ne.
+    - rewrite /interp_union => v.
+      rewrite !interp_car_simpl.
+      f_equiv.
+      + revert v; by apply hA.
+      + revert v; by apply hB.
+    - rewrite /interp_inter => v.
+      rewrite !interp_car_simpl.
+      f_equiv.
+      + revert v; by apply hA.
+      + revert v; by apply hB.
+    - rewrite /interp_tvar => v.
+      assert (hl: length x = length y) by now apply Forall2_length in h.
+      elim : x y tv h hl => [ | hd tl hi]; case => [ | hd' tl'] tv h /= hl => //.
+      apply Forall2_cons in h as [hhd htl].
+      case: tv hi => [ | tv ] hi //=.
+      apply:  hi; first done.
+      by lia.
+  Qed.
+
+  (* TODO: try to make this nicer by avoiding the pre definition of go/go_ne.
+   * Right now if we remove what's before, Coq can't find the _ne proof
+   * for the internal fixpoint
+   *)
+  Definition interp_type_pre (rec : ty_interpO) : ty_interpO :=
+    λ (typ : lang_ty), λne (env: listO (interpO Σ)), 
+    let go_rec : lang_ty → sem_typeO Σ :=
+    (fix go (typ: lang_ty) : interp Σ :=
+      match typ with
+      | IntT => interp_int
+      | BoolT => interp_bool
+      | NothingT => interp_nothing
+      | MixedT => interp_mixed env rec
+      | ClassT t targs =>
+          let env : list (interp Σ) := List.map go targs in
+          interp_class t env rec
+      | NullT => interp_null
+      | NonNullT => interp_nonnull env rec
+      | UnionT A B => interp_union (go A) (go B)
+      | InterT A B => interp_inter (go A) (go B)
+      | VarT tv => interp_tvar env tv
+      end)
+    in go_rec typ.
+
+  Global Instance interp_type_pre_persistent (rec: ty_interpO) :
+    ∀ t env v, Persistent (interp_type_pre rec t env v).
+  Proof. by move => ???; apply _. Qed.
+
+
+  Lemma interp_class_contractive cname env: Contractive (interp_class cname env). 
   Proof.
     rewrite /interp_class => n i1 i2 hdist v.
-    rewrite !interp_car_unfold.
+    rewrite !interp_car_simpl.
     f_equiv ; intro l.
     f_equiv; intro t.
     f_equiv; intro fields.
     f_equiv.
-    set (f := λ i, interp_fields i fields).
-    assert (hf : Contractive f) by apply interp_fields_contractive.
-    by apply (mapsto_contractive _ _ f).
+    rewrite mapsto_eq /mapsto_def /loc_mapsto_def.
+    do 3 f_equiv.
+    by apply interp_fields_contractive.
   Qed.
 
-  Lemma interp_nonnull_contractive: Contractive interp_nonnull.
+  Lemma interp_nonnull_contractive env: Contractive (interp_nonnull env).
   Proof.
     rewrite /interp_nonnull => n i1 i2 hdist v.
-    rewrite !interp_car_unfold.
+    rewrite !interp_car_simpl.
     do 4 f_equiv.
     revert v.
     by apply interp_class_contractive.
@@ -179,21 +288,31 @@ Section proofs.
   (* we cannot use solve_contractive out of the box because of
    * the 'fix' combinator above
    *)
-  Local Instance interp_type_pre_contractive:
-  Contractive (interp_type_pre).
+  Local Instance interp_type_pre_contractive : Contractive interp_type_pre.
   Proof.
-    move => n i1 i2 hdist.
-    move => ty.
-    elim : ty; intros; rewrite /interp_type_pre //=;
-    [ (* mixed *)| (*class*) | (*nonnull*) 
-    | solve_proper_core ltac:(fun _ => first [done | f_contractive | f_equiv])
-    | solve_proper_core ltac:(fun _ => first [done | f_contractive | f_equiv])
-    ].
-     - move => v; rewrite /interp_mixed !interp_car_unfold.
-       f_equiv; revert v.
-       by apply interp_nonnull_contractive.
-     - by apply interp_class_contractive.
-     - by apply interp_nonnull_contractive.
+    rewrite /interp_type_pre => n rec1 rec2 hdist ty env /=.
+    induction ty
+      as [ | | | | cname targs htargs | | | A B hA hB | A B hA hB | tv ]
+      using lang_ty_ind' => //=.
+    - rewrite /interp_mixed => v /=.
+      rewrite !interp_car_simpl.
+      f_equiv.
+      revert v; by apply interp_nonnull_contractive.
+    - move => v.
+      transitivity (interp_class cname (map (go env rec2) targs) rec1 v).
+      + revert v; apply interp_class_ne.
+        (* copied from _ne proof *)  
+        rewrite Forall_forall in htargs.
+        induction targs as [ | hd tl hi] => //=.
+        f_equiv.
+        { apply htargs.  by constructor. }
+        apply hi => ? hIn.
+        apply htargs.
+        now constructor.
+      + revert v; by apply interp_class_contractive.
+    - by apply interp_nonnull_contractive.
+    - solve_proper_core ltac:(fun _ => first [done | f_contractive | f_equiv]).
+    - solve_proper_core ltac:(fun _ => first [done | f_contractive | f_equiv]).
   Qed.
 
   (* the interpretation of types can now be
@@ -201,29 +320,31 @@ Section proofs.
      can be (mutually) recursive) *)
   Definition interp_type := fixpoint interp_type_pre.
 
-  Lemma interp_type_unfold (ty : lang_ty) (v : value) :
-    interp_type ty v ⊣⊢ interp_type_pre interp_type ty v.
+  Lemma interp_type_unfold (env: list (interpO Σ)) (ty : lang_ty) (v : value) :
+    interp_type ty env v ⊣⊢ interp_type_pre interp_type ty env v.
   Proof.
     rewrite {1}/interp_type.
-    apply (fixpoint_unfold interp_type_pre ty v).
+    apply (fixpoint_unfold interp_type_pre ty env v).
   Qed.
 
   (* #hyp *)
-  Global Instance interp_type_persistent : ∀ t v, Persistent (interp_type t v).
+  Global Instance interp_type_persistent :
+    ∀ t env v, Persistent (interp_type t env v).
   Proof.
-    elim => [ | | | | cname | | |s hs t ht | s hs t ht] v;
-        rewrite interp_type_unfold //=; try by apply _.
+    move => t env v.
+    rewrite interp_type_unfold.
+    by apply _.
   Qed.
 
-  Lemma dom_interp_fields fields:
-    dom stringset (interp_fields interp_type fields) ≡ dom _ fields.
+  Lemma dom_interp_fields env fields:
+    dom stringset (interp_fields env fields interp_type) ≡ dom _ fields.
   Proof. by rewrite /interp_fields dom_fmap. Qed.
 
   Lemma inherits_is_inclusion:
     ∀ A B, inherits A B →
-    ∀ v, interp_class A interp_type v -∗ interp_class B interp_type v.
+    ∀ env v, interp_class A env interp_type v -∗ interp_class B env interp_type v.
   Proof.
-    move => A B hAB v.
+    move => A B hAB env v.
     rewrite /interp_class.
     iIntros "h".
     iDestruct "h" as (ℓ t fields) "[%h hsem]".
@@ -240,22 +361,23 @@ Section proofs.
   (* A <: B → ΦA ⊂ ΦB *)
   Theorem subtype_is_inclusion_aux:
     ∀ (A B: lang_ty), A <: B →
-    ∀ v,
-    interp_type_pre interp_type A v -∗
-    interp_type_pre interp_type B v.
+    ∀ env v,
+    interp_type_pre interp_type A env v -∗
+    interp_type_pre interp_type B env v.
   Proof.
     induction 1 as [A | A B hext | | | | A | A B| A B | A B C h0 hi0 h1 hi1
         | A B | A B | A B C h0 hi0 h1 hi1 | A | A B C h0 hi0 h1 hi1 ];
-    move => v /=.
+    move => env v /=.
     - rewrite /interp_mixed.
       elim: A v => //=.
       + move => v; iIntros "h"; by repeat iLeft.
       + move => v; iIntros "h"; by iLeft; iRight; iLeft.
       + move => v; by rewrite /interp_nothing; iIntros "h".
-      + move => cname v.
+      + move => cname targs v.
         iIntros "h".
         iLeft; iRight; iRight.
-        iExists cname; by iApply inherits_is_inclusion. 
+        iExists cname. iApply inherits_is_inclusion. 
+        done.
       + move => v; iIntros "h"; by iRight.
       + move => v; by iIntros "h"; iLeft.
       + move => s hs t ht v.
